cedar-lean/Cedar/Thm/EntitySlice.lean
@@ -5,11 +5,259 @@ import Cedar.Thm.Entities
 import Cedar.Thm.Data.Map
 import Cedar.Thm.Validation.Typechecker.Types
 import Cedar.Validation.Types
+import Cedar.Thm.Validation.Typechecker
+import Cedar.Thm.Validation.Levels
+import Cedar.Thm.SubExpression
 
 namespace Cedar.Thm
 open Cedar.Data
 open Cedar.Validation
 open Cedar.Spec
+
+theorem append_membership {α : Type} (l₁ : List α) (l₂ : List α) (a : α) :
+  a ∈ (l₁ ++ l₂) →
+  a ∈ l₁ ∨ a ∈ l₂
+  := by
+  intros in_append
+  cases l₁
+  case nil =>
+    simp [List.append] at in_append
+    simp [in_append]
+  case cons head tail =>
+    cases in_append
+    case head =>
+      simp
+    case tail in_tail =>
+      have step : a ∈ tail ∨ a ∈ l₂ := by
+        apply append_membership
+        apply in_tail
+      rcases step with step | step
+        <;> simp [step]
+
+theorem in_joins_in_member {α : Type} (l : List (List α)) (a : α)
+  (in_lists : a ∈ l.join) :
+  ∃ l',
+    l' ∈ l ∧ a ∈ l'
+  := by
+  cases l
+  case nil =>
+    simp [List.join] at in_lists
+  case cons head tail =>
+    rw [List.join_cons] at in_lists
+    have step : a ∈ head ∨ a ∈ tail.join := by
+      apply append_membership
+      assumption
+    rcases step with step | step
+    case _ =>
+      exists head
+      constructor
+      · simp
+      · apply step
+    case _ =>
+      have step₂ : ∃ l', l' ∈ tail ∧ a ∈ l' := by
+        apply in_joins_in_member
+        assumption
+      replace ⟨l', step₂⟩ := step₂
+      exists l'
+      constructor <;> try simp
+      repeat simp [step₂]
+
+theorem in_joins_in_member' {α : Type} (head_list : List α) (tail_list : List (List α)) (a : α)
+  (in_lists : a ∈ (head_list :: tail_list).join) :
+  ∃ target_list,
+    a ∈ target_list ∧
+    (
+      target_list = head_list ∨ target_list ∈ tail_list
+    )
+  := by
+  have h := in_joins_in_member (head_list :: tail_list) a in_lists
+  replace ⟨target, h₁, h₂⟩ := h
+  clear h
+  exists target
+  simp [h₂]
+  cases h₁
+  case head =>
+    simp
+  case tail in_tail =>
+    apply Or.inr
+    apply in_tail
+
+
+
+
+
+
+
+def in_list_in_join {α : Type} (list : List α) (lists : List (List α)) (a : α)
+  (in_list : a ∈ list)
+  (in_lists : list ∈ lists) :
+  a ∈ lists.join
+  := by
+  exact List.mem_join_of_mem in_lists in_list
+
+
+def SimpleSliceContxtSoundness (v : Value) : Prop :=
+  ∀ euid edata (entities slice : Entities) (list : List (EntityUID × EntityData)),
+    v.findEuids entities = some list →
+    slice.find? euid = some edata →
+    (euid, edata) ∈ list →
+    slice.find? euid = entities.find? euid
+
+theorem simpleSlice_set (members : List Value) (euid : EntityUID) (edata : EntityData) (entities slice : Entities) (list : List (List (EntityUID × EntityData)))
+  (h : members.mapM (λ value => value.findEuids entities) = some list)
+  (in_slice : slice.find? euid = some edata)
+  (in_list : (euid, edata) ∈ list.join)
+  (ih : ∀ v, v ∈ members → SimpleSliceContxtSoundness v) :
+  slice.find? euid = entities.find? euid
+  := by
+  cases members
+  case nil =>
+    simp [List.mapM, List.mapM.loop] at h
+    subst h
+    simp [List.join] at in_list
+  case cons head tail =>
+    rw [List.mapM_cons] at h
+    cases find_in_head : head.findEuids entities
+    <;> simp [find_in_head] at h
+    cases find_in_tail : tail.mapM (λ value => value.findEuids entities)
+    <;> simp [find_in_tail] at h
+    rename_i head_list tail_list
+    have step : ∃ target_list,
+      (euid, edata) ∈ target_list ∧
+      (
+        target_list = head_list ∨ target_list ∈ tail_list
+      ) := by
+      apply in_joins_in_member'
+      rw [← h] at in_list
+      apply in_list
+    replace ⟨target_list, step₁, step₂⟩ := step
+    clear step
+    subst h
+    cases step₂
+    case _ step₂ =>
+      subst step₂
+      apply ih
+      simp
+      apply Or.inl
+      rfl
+      apply find_in_head
+      apply in_slice
+      apply step₁
+    case _ step₂ =>
+      apply simpleSlice_set
+      apply find_in_tail
+      apply in_slice
+      apply in_list_in_join
+      apply step₁
+      apply step₂
+      intros v in_tail
+      apply ih
+      simp [in_tail]
+
+
+
+theorem simpleSlice_context_value (v : Value) (euid : EntityUID) (edata : EntityData) (entities slice : Entities) (context_entities : List (EntityUID × EntityData))
+  (context_entities_def : v.findEuids entities = some context_entities)
+  (in_slice : slice.find? euid = some edata)
+  (in_context_entiites : (euid, edata) ∈ context_entities) :
+  slice.find? euid = entities.find? euid
+  := by
+  cases v
+  case prim p =>
+    cases p <;> try
+      (
+      simp [Value.findEuids, Prim.findEuids] at context_entities_def ;
+      subst context_entities_def
+      cases in_context_entiites
+      )
+    case entityUID euid' =>
+      simp [Value.findEuids, Prim.findEuids] at context_entities_def
+      cases find : entities.find? euid'
+        <;> simp [find] at context_entities_def
+      subst context_entities_def
+      cases in_context_entiites
+      case tail h =>
+        cases h
+      case head =>
+        simp [find, in_slice]
+  case set members =>
+    simp [Value.findEuids] at context_entities_def
+    simp [List.mapM₁, List.attach, List.attachWith] at context_entities_def
+    simp [List.mapM_pmap_subtype (λ (value : Value) => value.findEuids entities )] at context_entities_def
+    cases mapping : members.toList.mapM (λ value => value.findEuids entities)
+    <;> simp [mapping] at context_entities_def
+    rename_i list_of_lists
+    apply simpleSlice_set
+    apply mapping
+    apply in_slice
+    rw [← context_entities_def] at in_context_entiites
+    apply in_context_entiites
+    intros v in_values
+    apply simpleSlice_context_value
+  case record =>
+    sorry
+  case ext =>
+    sorry
+
+theorem simpleSlice_context (req : Request) (euid : EntityUID) (edata : EntityData) (entities slice : Entities) (context_entities : List (EntityUID × EntityData))
+  (context_entities_def : loadEuids req.context entities = some context_entities)
+  (in_slice : slice.find? euid = some edata)
+  (in_context_entiites : (euid, edata) ∈ context_entities) :
+  slice.find? euid = entities.find? euid
+  := by
+  simp [loadEuids] at context_entities_def
+
+
+
+  sorry
+
+
+theorem simpleSlice_is_subslice (req : Request) (entities slice : Entities)
+  (slice_def : simpleSlice req entities = some slice) :
+  subslice slice entities
+  := by
+  simp [subslice]
+  intros euid edata in_slice
+  simp [simpleSlice] at slice_def
+  cases find_principal : entities.find? req.principal
+    <;> simp [find_principal] at slice_def
+  cases find_action : entities.find? req.action
+    <;> simp [find_action] at slice_def
+  cases find_resource : entities.find? req.resource
+    <;> simp [find_resource] at slice_def
+  rename_i principal action resource
+  cases find_entities_in_context : (loadEuids req.context entities)
+    <;> simp [find_entities_in_context] at slice_def
+  rename_i context_entities
+  have location : (euid, edata) ∈ (req.principal, principal) :: (req.action, action) :: (req.resource, resource) :: context_entities := by
+    have in_kvs : (euid, edata) ∈ slice.kvs := by
+      exact Map.find_means_mem in_slice
+    apply Map.make_mem_list_mem
+    rw [slice_def]
+    assumption
+  cases location
+  -- It's the principal
+  simp [in_slice, find_principal]
+  rename_i location
+  cases location
+  -- It's the action
+  simp [in_slice, find_action]
+  rename_i location
+  cases location
+  -- It's the resource
+  simp [in_slice, find_resource]
+  rename_i location
+
+  apply simpleSlice_context
+  repeat assumption
+
+
+
+
+
+
+
+
 
 theorem simpleSlice_is_subslice (req : Request) (entities slice : Entities)
   (h : simpleSlice req entities = some slice) :
@@ -25,7 +273,7 @@ theorem simpleSlice_is_subslice (req : Request) (entities slice : Entities)
   cases find_resource : entities.find? req.resource
     <;> simp [find_resource] at h
   rename_i principal action resource
-  have location : (euid, edata) ∈ [(req.principal, principal), (req.action, action), (req.resource, resource)] := by
+  have location : (euid, edata) ∈ [(req.principal, principal),  (req.action, action),  (req.resource, resource)] := by
     have in_map : (euid, edata) ∈ slice.kvs := by
       exact Map.find_means_mem h'
     apply Map.make_mem_list_mem
@@ -45,9 +293,9 @@ theorem simpleSlice_is_subslice (req : Request) (entities slice : Entities)
   case _ =>
     rw [h']
     rw [find_resource]
-  case _ =>
-    rename_i location
-    cases location
+  rename_i location
+  cases location
+
 
 theorem simpleSlice_respects_entity_schema (req : Request) (entities slice : Entities) (env : Environment)
   (h₁ : simpleSlice req entities = some slice)
@@ -66,38 +314,200 @@ theorem simpleSlice_respects_entity_schema (req : Request) (entities slice : Ent
   apply h₂
   simp [in_full_store]
 
+def simpleSlice_soundness (e : Expr) : Prop  :=
+  ∀ entities slice request env (c₁ c₂ : Capabilities) (ty : CedarType),
+    typeOf e c₁ env (.finite 1 == Level.infinite) = .ok (ty, c₂) →
+    CapabilitiesInvariant c₁ request entities →
+    simpleSlice request entities = .some slice →
+    RequestAndEntitiesMatchEnvironmentLeveled env request entities (.finite 1)  →
+    evaluate e request slice = evaluate e request entities
 
-
-
-
-
-
-
-
-
-
-theorem simpleSlice_wf (req : Request) (entities slice : Entities) (env : Environment)
-  (h₁ : simpleSlice req entities = some slice)
-  (h₂ : InstanceOfRequestTypeLevel req env.reqty (.finite 1))
-  (h₃ : InstanceOfEntitySchema entities env.ets)
-  (h₃ : InstanceOfActionSchema entities env.acts)
-  :
-  RequestAndEntitiesMatchEnvironmentLeveled env request slice (.finite 1)
+theorem simpleSlice_sound_lit (l : Prim) (entities slice : Entities) (request : Request)  :
+  evaluate (.lit l) request slice = evaluate (.lit l) request entities
   := by
-  simp [RequestAndEntitiesMatchEnvironmentLeveled]
+  cases l <;> simp [evaluate]
+
+theorem simpleSlice_is_sound_var (v : Var) (entities slice : Entities) (request : Request)  :
+  evaluate (.var v) request slice = evaluate (.var v) request entities
+  := by
+  cases v <;> simp [evaluate]
+
+theorem one_is_less_than_infinity : Level.finite 1 < .infinite := by
+  apply LevelLT.finite₂
+
+theorem simpleSlice_is_sound_ite (cond cons alt : Expr) (entities slice : Entities) (request : Request) (env : Environment) (c₁ c₂ : Capabilities) (ty : CedarType)
+  (well_typed : typeOf (.ite cond cons alt) c₁ env (Level.finite 1 == .infinite) = .ok (ty, c₂))
+  (slice_eq : simpleSlice request entities = .some slice)
+  (caps_inv : CapabilitiesInvariant c₁ request entities)
+  (full_store_typed : RequestAndEntitiesMatchEnvironmentLeveled env request entities (.finite 1))
+  (ih₁ : simpleSlice_soundness cond)
+  (ih₂ : simpleSlice_soundness cons)
+  (ih₃ : simpleSlice_soundness alt) :
+  evaluate (.ite cond cons alt) request slice = evaluate (.ite cond cons alt) request entities
+  := by
+  simp [evaluate]
+  have ⟨bty, c₁', ty₁, c₂', ty₂, c₃, hinv₁, hinv₂⟩ := type_of_ite_inversion well_typed
+  cases bty
+  case tt =>
+    simp at hinv₂
+
+    have ⟨caps_inv_cond, v_cond, cond_sound, v_cond_typed⟩ : GuardedCapabilitiesInvariant cond c₁' request entities ∧ ∃ (v : Value), EvaluatesToLeveled cond request entities v ∧ InstanceOfType v (.bool .tt) := by
+      apply type_of_is_sound_noninfinite
+      apply one_is_less_than_infinity
+      repeat assumption
+    cases v_cond_typed
+    rename_i bool v_cond_typed
+    cases bool
+    <;> simp [InstanceOfBoolType] at v_cond_typed
+    have eval_cond_matches : evaluate cond request slice = evaluate cond request entities := by
+      apply ih₁
+      repeat assumption
+    rcases cond_sound with cond_sound | cond_sound | cond_sound
+      <;> simp [cond_sound, eval_cond_matches, Result.as, Coe.coe, Value.asBool]
+
+    replace ⟨hinv₂, hinv₃, hinv₄⟩ := hinv₂
+    subst hinv₃
+    subst hinv₄
+    apply ih₂
+    apply hinv₂
+    apply capability_union_invariant
+    assumption
+    apply caps_inv_cond
+    repeat assumption
+  case ff =>
+    simp at hinv₂
+    replace ⟨hinv₂, hinv₃, hinv₄⟩ := hinv₂
+    subst hinv₃
+    subst hinv₄
+
+    have ⟨caps_inv_cond, v_cond, cond_sound, v_cond_typed⟩ : GuardedCapabilitiesInvariant cond c₁' request entities ∧ ∃ (v : Value), EvaluatesToLeveled cond request entities v ∧ InstanceOfType v (.bool .ff) := by
+      apply type_of_is_sound_noninfinite
+      apply one_is_less_than_infinity
+      repeat assumption
+    cases v_cond_typed
+    rename_i bool v_cond_typed
+    cases bool
+    <;> simp [InstanceOfBoolType] at v_cond_typed
+    have eval_cond_matches : evaluate cond request slice = evaluate cond request entities := by
+      apply ih₁
+      repeat assumption
+    rcases cond_sound with cond_sound | cond_sound | cond_sound
+      <;> simp [cond_sound, eval_cond_matches, Result.as, Coe.coe, Value.asBool]
+    apply ih₃
+    repeat assumption
+  case anyBool =>
+    simp at hinv₂
+    have ⟨caps_inv_cond, v_cond, cond_sound, v_cond_typed⟩ : GuardedCapabilitiesInvariant cond c₁' request entities ∧ ∃ (v : Value), EvaluatesToLeveled cond request entities v ∧ InstanceOfType v (.bool .anyBool) := by
+      apply type_of_is_sound_noninfinite
+      apply one_is_less_than_infinity
+      repeat assumption
+
+    have eval_cond_matches : evaluate cond request slice = evaluate cond request entities := by
+      apply ih₁
+      repeat assumption
+
+
+    rcases cond_sound with cond_sound | cond_sound | cond_sound
+    <;> simp [cond_sound, eval_cond_matches, Result.as, Coe.coe, Value.asBool]
+    cases v_cond_typed
+    rename_i bool v_cond_typed
+    clear v_cond_typed
+    replace ⟨hinv₂, hinv₃, _⟩ := hinv₂
+    cases bool
+    case true =>
+      simp
+      apply ih₂
+      apply hinv₂
+      apply capability_union_invariant
+      assumption
+      apply caps_inv_cond
+      assumption
+      repeat assumption
+    case false =>
+      simp
+      apply ih₃
+      repeat assumption
+
+
+theorem simpleSlice_is_sound_getAttr (e : Expr) (attr : Attr) (entities slice : Entities) (request : Request) (env : Environment) (c₁ c₂ : Capabilities) (ty : CedarType)
+  (well_typed : typeOf (.getAttr e attr) c₁ env (.finite 1 == Level.infinite) = .ok (ty, c₂))
+  (slice_eq : simpleSlice request entities = .some slice)
+  (caps_inv : CapabilitiesInvariant c₁ request entities)
+  (full_store_typed : RequestAndEntitiesMatchEnvironmentLeveled env request entities (.finite 1))
+  (ih : simpleSlice_soundness e)
+  :
+  evaluate (.getAttr e attr) request slice = evaluate (.getAttr e attr) request entities
+  := by
+  simp [evaluate]
+
+  have ⟨hinv₁, c₁', hinv₂⟩ := type_of_getAttr_inversion_levels well_typed
+  cases hinv₂
+  case _ hinv₂ => -- entity case
+    replace ⟨etype, l₂, hinv₂, hinv₃⟩ := hinv₂
+    have ⟨caps_inv_subexpr, v, sound_subexpr, v_well_typed⟩ : GuardedCapabilitiesInvariant e c₁' request entities ∧ ∃ v, EvaluatesToLeveled e request entities v ∧ InstanceOfType v (.entity etype l₂) := by
+      apply type_of_is_sound_noninfinite
+      apply one_is_less_than_infinity
+      repeat assumption
+    have eval_matches : evaluate e request slice = evaluate e request entities := by
+      apply ih
+      repeat assumption
+    rcases sound_subexpr with sound_subexpr | sound_subexpr | sound_subexpr
+    <;> simp [sound_subexpr, eval_matches]
 
 
 
+
+
+
+
+    sorry
+  case _ =>
+    sorry
+
+
+
+
+
+
+
+
+
+theorem simpleSlice_is_sound (e : Expr) (entities slice : Entities) (request : Request) (env : Environment) (c₁ c₂ : Capabilities) (ty : CedarType)
+  (well_typed : typeOf e c₁ env false = .ok (ty, c₂))
+  (slice_eq : simpleSlice request entities = .some slice)
+  (caps_inv : CapabilitiesInvariant c₁ request entities)
+  (full_store_typed : RequestAndEntitiesMatchEnvironmentLeveled env request entities (.finite 1)) :
+  evaluate e request slice = evaluate e request entities
+  := by
+  cases e
+  case lit l =>
+    apply simpleSlice_sound_lit
+  case var v =>
+    apply simpleSlice_is_sound_var
+  case ite cond cons alt =>
+    apply simpleSlice_is_sound_ite
+    repeat assumption
+    case _ =>
+      simp [simpleSlice_soundness]
+      intros
+      apply simpleSlice_is_sound
+      repeat assumption
+    case _ =>
+      simp [simpleSlice_soundness]
+      intros
+      apply simpleSlice_is_sound
+      repeat assumption
+    case _ =>
+      simp [simpleSlice_soundness]
+      intros
+      apply simpleSlice_is_sound
+      repeat assumption
+  case and lhs rhs =>
+    sorry
+  case or lhs rhs =>
+    sorry
+  case getAttr expr attr =>
+    sorry
 
 
   sorry
-
-
-
-
-
-
-
-
-
-end Cedar.Thm
