cedar-lean/Cedar/Thm/SubExpression.lean
@@ -1,0 +1,38 @@
+import Cedar.Spec.Value
+import Cedar.Data.Map
+import Cedar.Data.List
+
+namespace Cedar.Thm
+open Cedar.Data
+open Cedar.Spec
+
+
+inductive InValue : Value → Value → Prop :=
+  | inSet : ∀ v vs,
+    v ∈ vs →
+    InValue v (.set vs)
+  | inRecord : ∀ k v kvs,
+    kvs.find? k = some v →
+    InValue v (.record kvs)
+
+inductive SubValue : Value → Value → Prop :=
+  | refl : ∀ v, SubValue v v
+  | direct : ∀ v v',
+    InValue v v' →
+    SubValue v v'
+  | trans : ∀ a b c,
+    SubValue a b →
+    SubValue b c →
+    SubValue a c
+
+def SubValue.inSet v vs (h : v ∈ vs) : SubValue v (.set vs) := by
+  apply SubValue.direct
+  apply InValue.inSet
+  assumption
+
+def SubValue.inRecord k v kvs (h : kvs.find? k = some v ) : SubValue v (.record kvs) := by
+  apply SubValue.direct
+  apply InValue.inRecord
+  assumption
+
+end Cedar.Thm
